Sequences/NatSeqConversions.dfy
@@ -5,37 +5,37 @@ abstract module NatSeqConversions refines NatSeq {
   import NatSeq1
   import NatSeq2
 
-  /* BASE2() to the power of P() is BASE1(). */
-  function P(): nat
+  /* NatSeq2.BASE() to the power of E() is NatSeq1.BASE(). */
+  function E(): nat
   {
     var n: nat :| NatSeq1.BASE() == power(NatSeq2.BASE(), n) && n > 1;
     n
   }
 
-  /* Converts a sequence from BASE1() to BASE2(). */
+  /* Converts a sequence from NatSeq1.BASE() to NatSeq2.BASE(). */
   function {:opaque} to_lower_base(xs: seq<NatSeq1.uint>): seq<NatSeq2.uint>
   {
     if |xs| == 0 then []
-    else NatSeq2.to_seq_with_len(first(xs), P()) + to_lower_base(drop_first(xs))
+    else NatSeq2.to_seq_with_len(first(xs), E()) + to_lower_base(drop_first(xs))
   }
 
-  /* Converts a sequence from BASE2() to BASE1(). */
+  /* Converts a sequence from NatSeq2.BASE() to NatSeq1.BASE(). */
   function {:opaque} to_higher_base(xs: seq<NatSeq2.uint>): seq<NatSeq1.uint>
   {
     if |xs| == 0 then []
     else
-      if |xs| < P() then
+      if |xs| < E() then
         NatSeq2.lemma_seq_nat_bound(xs);
-        lemma_power_strictly_increases(NatSeq2.BASE(), |xs|, P());
+        lemma_power_strictly_increases(NatSeq2.BASE(), |xs|, E());
         [NatSeq2.to_nat(xs) as NatSeq1.uint]
       else
-        NatSeq2.lemma_seq_nat_bound(xs[..P()]);
+        NatSeq2.lemma_seq_nat_bound(xs[..E()]);
         lemma_mod_sub_multiples_vanish_auto();
-        [NatSeq2.to_nat(xs[..P()]) as NatSeq1.uint] + to_higher_base(xs[P()..])
+        [NatSeq2.to_nat(xs[..E()]) as NatSeq1.uint] + to_higher_base(xs[E()..])
   }
 
-  /* Sequence conversion from BASE1() to BASE2() does not change its nat
-  representation. */
+  /* Sequence conversion from NatSeq1.BASE() to NatSeq2.BASE() does not change
+  its nat representation. */
   lemma lemma_lower_base_to_nat(xs: seq<NatSeq1.uint>)
     ensures NatSeq2.to_nat(to_lower_base(xs)) == NatSeq1.to_nat(xs)
   {
@@ -45,39 +45,37 @@ abstract module NatSeqConversions refines NatSeq {
     if |xs| > 0 {
       calc {
         NatSeq2.to_nat(to_lower_base(xs));
-        NatSeq2.to_nat(NatSeq2.to_seq_with_len(first(xs), P()) + to_lower_base(drop_first(xs)));
-          { NatSeq2.lemma_seq_prefix(NatSeq2.to_seq_with_len(first(xs), P())
-            + to_lower_base(drop_first(xs)), P()); }
-        NatSeq2.to_nat(NatSeq2.to_seq_with_len(first(xs), P())) + NatSeq2.to_nat(to_lower_base(drop_first(xs))) * power(NatSeq2.BASE(), P());
+        NatSeq2.to_nat(NatSeq2.to_seq_with_len(first(xs), E()) + to_lower_base(drop_first(xs)));
+          { NatSeq2.lemma_seq_prefix(NatSeq2.to_seq_with_len(first(xs), E()) + to_lower_base(drop_first(xs)), E()); }
+        NatSeq2.to_nat(NatSeq2.to_seq_with_len(first(xs), E())) + NatSeq2.to_nat(to_lower_base(drop_first(xs))) * power(NatSeq2.BASE(), E());
           {
-            NatSeq2.lemma_to_seq_with_len_eq_to_seq(first(xs), P());
+            NatSeq2.lemma_to_seq_with_len_eq_to_seq(first(xs), E());
             NatSeq2.lemma_nat_seq_nat(first(xs));
             lemma_lower_base_to_nat(drop_first(xs));
           }
-        first(xs) + NatSeq1.to_nat(drop_first(xs)) * power(NatSeq2.BASE(), P());
-          { assert power(NatSeq2.BASE(), P()) == NatSeq1.BASE(); }
+        first(xs) + NatSeq1.to_nat(drop_first(xs)) * power(NatSeq2.BASE(), E());
+          { assert power(NatSeq2.BASE(), E()) == NatSeq1.BASE(); }
         NatSeq1.to_nat(xs);
       }
     }
   }
 
-  /* Sequence conversion from BASE2() to BASE1() does not change its nat
-  representation. */
+  /* Sequence conversion from NatSeq2.BASE() to NatSeq1.BASE() does not change
+  its nat representation. */
   lemma lemma_higher_base_to_nat(xs: seq<NatSeq2.uint>)
     ensures NatSeq1.to_nat(to_higher_base(xs)) == NatSeq2.to_nat(xs)
   {
     reveal NatSeq1.to_nat();
     reveal NatSeq2.to_nat();
     reveal to_higher_base();
-    if |xs| >= P() {
+    if |xs| >= E() {
       calc {
         NatSeq1.to_nat(to_higher_base(xs));
-          { NatSeq2.lemma_seq_nat_bound(xs[..P()]); }
-        NatSeq1.to_nat([NatSeq2.to_nat(xs[..P()]) as NatSeq1.uint] + to_higher_base(xs[P()..]));
-        NatSeq2.to_nat(xs[..P()]) as NatSeq1.uint + NatSeq1.to_nat(to_higher_base(xs[P()..])) * NatSeq1.BASE();
-          { lemma_higher_base_to_nat(xs[P()..]); }
-        NatSeq2.to_nat(xs[..P()]) + NatSeq2.to_nat(xs[P()..]) * power(NatSeq2.BASE(), P());
-          { NatSeq2.lemma_seq_prefix(xs, P()); }
+          { NatSeq2.lemma_seq_nat_bound(xs[..E()]); }
+        NatSeq1.to_nat([NatSeq2.to_nat(xs[..E()]) as NatSeq1.uint] + to_higher_base(xs[E()..]));
+          { lemma_higher_base_to_nat(xs[E()..]); }
+        NatSeq2.to_nat(xs[..E()]) + NatSeq2.to_nat(xs[E()..]) * power(NatSeq2.BASE(), E());
+          { NatSeq2.lemma_seq_prefix(xs, E()); }
         NatSeq2.to_nat(xs);
       }
     }
